michael_formal/not4afp/Paper_Example.thy
@@ -156,7 +156,7 @@ proof-
      by (simp add: possible_steps_def ffilter_def set_filter abs_fset)
  qed
 
-lemma drinks_before_1_invalid: "\<not>(aa = ''coin'' \<and> b = [Num 50]) \<Longrightarrow> nondeterministic_step drinks_before 1 r aa b = None"
+lemma drinks_before_1_invalid: "\<not> (aa = ''coin'' \<and> b = [Num 50]) \<Longrightarrow> nondeterministic_step drinks_before 1 r aa b = None"
 proof-
   assume premise: "\<not>(aa = ''coin'' \<and> b = [Num 50])"
   have set_filter: "(Set.filter
@@ -231,12 +231,224 @@ proof-
     by auto
 qed
 
+lemma possible_steps_drinks_before_coin: "length b = 1 \<Longrightarrow> possible_steps drinks_before 2 r1 ''coin'' b = {|(2, coin)|}"
+proof-
+  assume premise: "length b = 1"
+  have set_filter: "(Set.filter
+       (\<lambda>((origin, dest), t).
+           origin = 2 \<and>
+           Label t = ''coin'' \<and> length b = Arity t \<and> apply_guards (Guard t) (case_vname (\<lambda>n. input2state b 1 (I n)) (\<lambda>n. r1 (R n))))
+       (fset drinks_before)) = {((2, 2), coin)}"
+    apply (simp add: drinks_before_def Set.filter_def)
+    apply safe
+    by (simp_all add: transitions premise)
+  show ?thesis
+    by (simp add: possible_steps_def ffilter_def set_filter)
+qed
+
+lemma possible_steps_merge_1_2_update_coin: "length b = 1 \<Longrightarrow> (1, coin) |\<in>| possible_steps merge_1_2_update 1 r2 ''coin'' b"
+proof-
+  assume premise: "length b = 1"
+  have set_filter: "((1, 1), coin) \<in> (Set.filter
+       (\<lambda>((origin, dest), t).
+           origin = 1 \<and>
+           Label t = ''coin'' \<and> length b = Arity t \<and> apply_guards (Guard t) (case_vname (\<lambda>n. input2state b 1 (I n)) (\<lambda>n. r2 (R n))))
+       (fset merge_1_2_update))"
+    apply (simp add: merge_1_2_update_def Set.filter_def)
+    apply safe
+    by (simp_all add: transitions premise)
+  show ?thesis
+    apply (simp add: possible_steps_def ffilter_def)
+    using set_filter
+    by (metis (no_types, lifting) case_prod_conv ffilter.rep_eq fimage_eqI fset_inverse notin_fset)
+qed
+
+lemma nondeterministic_step_drinks_before_invalid_step_2: " \<not> (aa = ''coin'' \<and> length b = 1) \<Longrightarrow>
+       \<not> (aa = ''vend'' \<and> b = []) \<Longrightarrow> nondeterministic_step drinks_before 2 r1 aa b = None"
+proof-
+  assume premise1:  "\<not> (aa = ''coin'' \<and> length b = 1)"
+  assume premise2: "\<not> (aa = ''vend'' \<and> b = [])"
+  have set_filter: "(Set.filter
+           (\<lambda>((origin, dest), t).
+               origin = 2 \<and>
+               Label t = aa \<and> length b = Arity t \<and> apply_guards (Guard t) (case_vname (\<lambda>n. input2state b 1 (I n)) (\<lambda>n. r1 (R n))))
+           (fset drinks_before)) = {}"
+    using premise1 premise2
+    apply (simp add: Set.filter_def drinks_before_def)
+    apply safe
+    by (simp_all add: transitions)
+  show ?thesis
+    apply (simp add: nondeterministic_step_def possible_steps_def ffilter_def set_filter)
+    using bot_fset_def by force
+qed
+
+lemma impossible_steps_drinks_before_vend: "\<nexists>n. r (R 2) = Some (Num n) \<Longrightarrow> nondeterministic_step drinks_before 2 r ''vend'' i = None"
+proof-
+  assume premise: "\<nexists>n. r (R 2) = Some (Num n)"
+  have set_filter: "(Set.filter
+       (\<lambda>((origin, dest), t).
+           origin = 2 \<and>
+           Label t = ''vend'' \<and> length i = Arity t \<and> apply_guards (Guard t) (case_vname (\<lambda>n. input2state i 1 (I n)) (\<lambda>n. r (R n))))
+       (fset drinks_before)) = {}"
+    using premise
+    apply (simp add: Set.filter_def drinks_before_def)
+    apply safe
+      apply (simp add: transitions)
+     apply (simp add: transitions)
+     apply (metis MaybeBoolInt.elims option.simps(3))
+     apply (simp add: transitions)
+    apply (case_tac "MaybeBoolInt (\<lambda>x y. y < x) (Some (Num 100)) (r (R 2))")
+     apply simp
+    apply simp
+    by (metis MaybeBoolInt.elims option.simps(3))
+  show ?thesis
+    apply (simp add: nondeterministic_step_def possible_steps_def ffilter_def set_filter)
+    using bot_fset_def by force
+qed
+
+lemma drinks_before_vend_fail: "r (R 2) = Some (Num x1) \<Longrightarrow> x1 < 100 \<Longrightarrow> possible_steps drinks_before 2 r ''vend'' [] = {|(2, vend_fail)|}"
+proof-
+  assume premise1: "r (R 2) = Some (Num x1)"
+  assume premise2: "x1 < 100"
+  have set_filter: "(Set.filter
+       (\<lambda>((origin, dest), t).
+           origin = 2 \<and> Label t = ''vend'' \<and> Arity t = 0 \<and> apply_guards (Guard t) (case_vname (\<lambda>n. input2state [] 1 (I n)) (\<lambda>n. r (R n))))
+       (fset drinks_before)) = {((2, 2), vend_fail)}"
+    using premise1 premise2
+    apply (simp add: Set.filter_def drinks_before_def)
+    apply safe
+    by (simp_all add: transitions)
+  show ?thesis
+    by (simp add: possible_steps_def ffilter_def set_filter)
+qed
+
+lemma drinks_before_vend_success: "r (R 2) = Some (Num x1) \<Longrightarrow> x1 \<ge> 100 \<Longrightarrow> possible_steps drinks_before 2 r ''vend'' [] = {|(3, vend_success)|}"
+proof-
+  assume premise1: "r (R 2) = Some (Num x1)"
+  assume premise2: "x1 \<ge> 100"
+  have set_filter: "(Set.filter
+       (\<lambda>((origin, dest), t).
+           origin = 2 \<and> Label t = ''vend'' \<and> Arity t = 0 \<and> apply_guards (Guard t) (case_vname (\<lambda>n. input2state [] 1 (I n)) (\<lambda>n. r (R n))))
+       (fset drinks_before)) = {((2, 3), vend_success)}"
+    using premise1 premise2
+    apply (simp add: Set.filter_def drinks_before_def)
+    apply safe
+    by (simp_all add: transitions)
+  show ?thesis
+    by (simp add: possible_steps_def ffilter_def set_filter)
+qed
+
+lemma merge_1_2_update_vend_fail: "r (R 2) = Some (Num x1) \<Longrightarrow> x1 < 100 \<Longrightarrow> possible_steps merge_1_2_update 1 r ''vend'' [] = {|(1, vend_fail)|}"
+  proof-
+  assume premise1: "r (R 2) = Some (Num x1)"
+  assume premise2: "x1 < 100"
+  have set_filter: "(Set.filter
+       (\<lambda>((origin, dest), t).
+           origin = 1 \<and> Label t = ''vend'' \<and> Arity t = 0 \<and> apply_guards (Guard t) (case_vname (\<lambda>n. input2state [] 1 (I n)) (\<lambda>n. r (R n))))
+       (fset merge_1_2_update)) = {((1, 1), vend_fail)}"
+    using premise1 premise2
+    apply (simp add: Set.filter_def merge_1_2_update_def)
+    apply safe
+    by (simp_all add: transitions)
+  show ?thesis
+    by (simp add: possible_steps_def ffilter_def set_filter)
+qed
+
+lemma merge_1_2_update_vend_success: "r (R 2) = Some (Num x1) \<Longrightarrow> x1 \<ge> 100 \<Longrightarrow> possible_steps merge_1_2_update 1 r ''vend'' [] = {|(3, vend_success)|}"
+  proof-
+  assume premise1: "r (R 2) = Some (Num x1)"
+  assume premise2: "x1 \<ge> 100"
+  have set_filter: "(Set.filter
+       (\<lambda>((origin, dest), t).
+           origin = 1 \<and> Label t = ''vend'' \<and> Arity t = 0 \<and> apply_guards (Guard t) (case_vname (\<lambda>n. input2state [] 1 (I n)) (\<lambda>n. r (R n))))
+       (fset merge_1_2_update)) = {((1, 3), vend_success)}"
+    using premise1 premise2
+    apply (simp add: merge_1_2_update_def Set.filter_def)
+    apply safe
+    by (simp_all add: transitions)
+  show ?thesis
+    by (simp add: possible_steps_def ffilter_def set_filter)
+qed
+
+lemma drinks_before_ends_at_3: "nondeterministic_step drinks_before 3 r aa b = None"
+proof-
+  have set_filter: "(Set.filter
+           (\<lambda>((origin, dest), t).
+               origin = 3 \<and>
+               Label t = aa \<and> length b = Arity t \<and> apply_guards (Guard t) (case_vname (\<lambda>n. input2state b 1 (I n)) (\<lambda>n. r (R n))))
+           (fset drinks_before)) = {}"
+    by (simp add: drinks_before_def Set.filter_def)
+  show ?thesis
+    apply (simp add: nondeterministic_step_def possible_steps_def ffilter_def set_filter)
+    using bot_fset_def by force
+qed
+
+lemma simulation_2_1: "\<forall>r. nondeterministic_simulates_trace drinks_before merge_1_2_update 2 1 r r lst"
+proof (induct lst)
+  case Nil
+  then show ?case
+    by (simp add: nondeterministic_simulates_trace.base)
+next
+  case (Cons a lst)
+  then show ?case
+    apply (case_tac a)
+    apply simp
+     apply (rule allI)
+    apply (case_tac "aa = ''coin'' \<and> length b = 1")
+     apply simp
+     apply (rule nondeterministic_simulates_trace.step_some)
+        apply (simp add: nondeterministic_step_def possible_steps_drinks_before_coin)
+    using possible_steps_merge_1_2_update_coin
+       apply blast
+      apply simp
+     apply simp
+    apply (case_tac "aa = ''vend'' \<and> b = []")
+     defer
+     apply (rule nondeterministic_simulates_trace.step_none)
+    using nondeterministic_step_drinks_before_invalid_step_2
+     apply blast
+    apply simp
+    apply (case_tac "r (R 2)")
+     apply (rule nondeterministic_simulates_trace.step_none)
+     apply (simp add: impossible_steps_drinks_before_vend)
+    apply (case_tac aaa)
+     defer
+     apply (rule nondeterministic_simulates_trace.step_none)
+     apply (simp add: impossible_steps_drinks_before_vend)
+    apply clarify
+    apply simp
+    apply (case_tac "x1 < 100")
+     apply (rule nondeterministic_simulates_trace.step_some)
+        apply (simp add: nondeterministic_step_def drinks_before_vend_fail)
+       apply (simp add: merge_1_2_update_vend_fail)
+      apply simp
+     apply (simp add: vend_fail_def)
+     apply (rule nondeterministic_simulates_trace.step_some)
+       apply (simp add: nondeterministic_step_def drinks_before_vend_success)
+      apply (simp add: merge_1_2_update_vend_success)
+     apply simp
+    apply (simp add: vend_success_def)
+    apply (case_tac lst)
+     apply (simp add: nondeterministic_simulates_trace.base)
+    apply simp
+    apply clarify
+    apply (rule nondeterministic_simulates_trace.step_none)
+    by (simp add: drinks_before_ends_at_3)
+  qed
+
 lemma simulation_1_1: "nondeterministic_simulates_trace drinks_before merge_1_2_update 1 1 <R 1 := d> <R 1 := d, R 2 := Num 0> ((aa, b) # list)"
 proof-
   have choice_coin50_coin: "(\<exists>a b. a = 1 \<and> b = coin50 \<or> a = 1 \<and> b = coin)"
     by auto
-  have abs_fset_empty: "Abs_fset {} = {||}"
-    by (simp add: bot_fset_def)
+  have coin50_updates: "(EFSM.apply_updates (Updates coin50)
+       (case_vname (\<lambda>n. if n = 1 then Some (Num 50) else input2state [] (1 + 1) (I n)) (\<lambda>n. if n = 1 then Some d else None)) <R 1 := d>) = 
+        <R 1 := d, R 2 := Num 50>"
+    apply (rule ext)
+    by (simp add: coin50_def)
+  have coin50_updates_2: "(EFSM.apply_updates (Updates coin50) (\<lambda>x. case x of I n \<Rightarrow> input2state [Num 50] 1 (I n) | R n \<Rightarrow> <R 1 := d, R 2 := Num 0> (R n))
+       <R 1 := d, R 2 := Num 0>) = <R 1 := d, R 2 := Num 50>"
+    apply (rule ext)
+    by (simp add: coin50_def)
   have set_filter: "\<forall>b d. (Set.filter
             (\<lambda>((origin, dest), t).
                 origin = 1 \<and>
@@ -250,21 +462,21 @@ proof-
     apply (case_tac "aa = ''coin'' \<and> b = [Num 50]")
      prefer 2
      apply (rule nondeterministic_simulates_trace.step_none)
-      apply (simp add: drinks_before_1_invalid)
+    using drinks_before_1_invalid
+    apply auto[1]
     
     apply (rule nondeterministic_simulates_trace.step_some)
      apply (simp add: nondeterministic_step_def possible_steps_drinks_before_coin_50)
-    apply (rule_tac x=coin50 in exI)
-    apply (simp add: nondeterministic_step_def merge_1_2_update_possible_steps_coin_50 choice_coin50_coin)
-    apply safe
-
-    sorry
+      apply (simp add: nondeterministic_step_def merge_1_2_update_possible_steps_coin_50 choice_coin50_coin)
+      apply auto[1]
+     apply simp
+    apply (simp add: coin50_updates coin50_updates_2)
+    by (simp add: simulation_2_1)
 qed
 
 lemma simulation_0_0: "nondeterministic_simulates_trace drinks_before merge_1_2_update 0 0 Map.empty Map.empty ((aa, b) # t)"
 proof-
-  have select_updates: "length b = 1 \<Longrightarrow> (\<lambda>x. if x = R 1 then aval (snd (R 1, V (I 1))) (case_vname (\<lambda>n. input2state b 1 (I n)) Map.empty)
-          else EFSM.apply_updates [] (case_vname (\<lambda>n. input2state b 1 (I n)) Map.empty) Map.empty x) = <R 1 := hd b>"
+  have select_updates: "length b = 1 \<Longrightarrow> (EFSM.apply_updates (Updates select) (case_vname (\<lambda>n. input2state b 1 (I n)) Map.empty) Map.empty) = <R 1 := hd b>"
     apply (rule ext)
     by (simp add: hd_input2state select_def)
   have select_update_updates: "length b = 1 \<Longrightarrow> (\<lambda>x. if x = R 1 then aval (snd (R 1, V (I 1))) (case_vname (\<lambda>n. input2state b 1 (I n)) Map.empty)
@@ -275,13 +487,11 @@ proof-
   apply (case_tac "aa = ''select'' \<and> length b = 1")
    apply (rule nondeterministic_simulates_trace.step_some)
      apply (simp add: nondeterministic_step_def possible_steps_drinks_before_select)
-    apply (simp add: nondeterministic_step_def possible_steps_merge_1_2_update_select transitions)
+       apply (simp add: nondeterministic_step_def possible_steps_merge_1_2_update_select transitions)
+    apply simp
    defer
    apply (rule nondeterministic_simulates_trace.step_none)
      apply (simp add: drinks_before_step_0_invalid)
-    apply safe
-      apply simp
-     apply simp
     apply (simp add: select_updates select_update_updates)
     apply (case_tac t)
      apply (simp add: nondeterministic_simulates_trace.base)
@@ -289,7 +499,7 @@ proof-
     by (simp add: simulation_1_1)
 qed
 
-lemma simulation_aux: "nondeterministic_simulates_trace merge_1_2 merge_1_2_update 0 0 Map.empty Map.empty t"
+lemma simulation_aux: "nondeterministic_simulates_trace drinks_before merge_1_2_update 0 0 Map.empty Map.empty t"
 proof (induct t)
 case Nil
   then show ?case
@@ -298,10 +508,11 @@ next
   case (Cons a t)
   then show ?case
     apply (case_tac a)
+    apply simp
     by (simp add: simulation_0_0)
 qed
 
-lemma simulation: "nondeterministic_simulates merge_1_2 merge_1_2_update"
+lemma simulation: "nondeterministic_simulates drinks_before merge_1_2_update"
   apply (simp add:nondeterministic_simulates_def)
   apply (rule allI)
   by (simp add: simulation_aux)
